TNF.v
@@ -1,8 +1,12 @@
 Require Import List.
+Require Import Lia.
+Require Import ZArith.
 
 From BusyCoq Require Import BB52Statement.
 From BusyCoq Require Import Prelims.
 From BusyCoq Require Import CustomTactics.
+From BusyCoq Require Import TM_CoqBB5.
+From BusyCoq Require Import Encodings.
 
 Section TNF.
 
